

Homework 6

Tejas Patel

10 November, 2025

12.1

6

$$f = \{(x, 4x + 5) : x \in \mathbb{Z}\}$$

The domain is \mathbb{Z}

Codomain is \mathbb{Z} , since all outputs are integers

Range is $4\mathbb{Z} + 5$

10

Yes (x^3, x) is a function from \mathbb{R} to \mathbb{R}

Every input has exactly one output and all inputs and outputs are real numbers

12.2

Injective is 1-1, Surjective is onto

6

$$(3n - 4m)$$

The function is surjective, with every value of \mathbb{Z} being mapped to a linear combination of 3 and -4

It is not injective as the counterexamples are $(4, 3)$ and $(8, 6)$

9

NOT COMPLETE

10

$$f(x) = \left(\frac{x+1}{x-1}\right)^3 \text{ is defined for all } x \neq 1$$

Solving for x we get $x = \frac{\sqrt[3]{f(x)}}{\sqrt[3]{f(x)} - 1}$, which is also defined for all $f(x), f(x) \neq -1$, meaning the function is surjective.

$$\text{Take } \frac{x_1 + 1}{x_1 - 1} = \frac{x_2 + 1}{x_2 - 1}$$

$$(x_1 + 1)(x_2 - 1) = (x_2 + 1)(x_1 - 1)$$

$$x_1x_2 - x_1 + x_2 - 1 = x_1x_2 - x_2 + x_1 - 1$$

$$x_2 - x_1 = x_1 - x_2 \text{ which is only true when } x_1 = x_2$$

18

We have $f(n) = \frac{(-1)^n(2n-1)+1}{4}$.

For n even, $(-1)^n = 1$ so $f(n) = \frac{n}{2}$, giving the nonnegative integers.

For n odd, $(-1)^n = -1$ so $f(n) = \frac{1-n}{2}$, giving the nonpositive integers. Both parts are strictly monotone and do not overlap, so f is injective.

For surjectivity, let $k \in \mathbb{Z}$. If $k \geq 0$, set $n = 2k$. Then $f(2k) = k$. If $k \leq 0$, set $n = 1 - 2k$. Then $f(1 - 2k) = k$. Every integer has a preimage, so f is surjective.

Therefore f is bijective.

12.4

3

$$g \cdot f = \{(1, 1), (2, 2), (3, 2)\}$$

$$f \cdot g = \{(1, 1), (2, 1), (3, 3)\}$$

4

$$g \cdot f = \{(a, a), (b, a), (c, a)\}$$

$$f \cdot g = \{(a, c), (b, c), (c, c)\}$$

5

$$g \cdot f = x + 1$$

$$f \cdot g = \sqrt[3]{x^3 + 1}$$

6

$$g \cdot f = \frac{3}{x^2 + 1} + 2$$

$$f \cdot g = \frac{1}{(3x + 2)^2 + 1}$$

10

$$f(x, y) = (xy, x^3)$$

$$(f \cdot f)(x, y) = f(f(x, y))$$

$$= f(x \cdot y, x^3)$$

$$= (x \cdot y \cdot x^3, (x \cdot y)^3)$$

$$= (x^4 y, x^3 y^3)$$

12.5

1

Let $y = f(n)$ and $x = n$

$$y = 6 - x.$$

Injective: If $f(a) = f(b)$, then $6 - a = 6 - b$, so $a = b$. Injective.

Surjective: For any $y \in \mathbb{R}$, solve $y = 6 - x$ to get $x = 6 - y$. Always real. Surjective.

So f is bijective.

Inverse: $y = 6 - x$ rearranges to $x = 6 - y$, so $f^{-1}(x) = 6 - x$.

2

$$y = \frac{5x-1}{x-2}.$$

Injective: Assume $f(a) = f(b)$: $\frac{5a-1}{a-2} = \frac{5b-1}{b-2}$. Cross-multiplying and simplifying yields $a = b$. Injective.

Surjective: Solve $y = \frac{5x-1}{x-2}$: $xy - 2y = 5x - 1$, $xy - 5x = 2y - 1$, $x(y - 5) = 2y - 1$, so $x = \frac{2y-1}{y-5}$. This works for all $y \neq 5$, so f is surjective onto $\mathbb{R} \setminus \{5\}$.

Thus $f: \mathbb{R} \setminus \{2\} \rightarrow \mathbb{R} \setminus \{5\}$ is bijective.

Inverse: $f^{-1}(x) = \frac{2x-1}{x-5}.$

3

Let $y = f(n)$ and $x = n$

$$y = 2^x.$$

Injective: $2^a = 2^b$ implies $a = b$ since the exponential is strictly increasing. Injective.

Surjective: Codomain is $(0, \infty)$. For any $y > 0$, solving $y = 2^x$ gives $x = \log_2(y)$. Surjective.

So $f: \mathbb{R} \rightarrow (0, \infty)$ is bijective.

Inverse: $f^{-1}(x) = \log_2(x).$

4

$$y = e^{(x^3+1)}$$

$$\ln(y) = x^3 + 1$$

$$\ln(y) - 1 = x^3$$

$$x = \sqrt[3]{\ln(y) - 1} \Rightarrow$$

$$y = \sqrt[3]{\ln(x) - 1}$$

6

Given $(x, y) = f(m, n)$, we solve $5m + 4n = x$ and $4m + 3n = y$. Subtracting $3(5m + 4n) = 3x$ from $4(4m + 3n) = 4y$ gives $m = 4y - 3x$. Substituting into $4m + 3n = y$ yields $n = 4x - 5y$. Thus $f^{-1}(x, y) = (4y - 3x, 4x - 5y)$

12.6

1

$$f(x) = x^2 + 3 \quad f'(x) = 2x$$

$$2x = 0 \text{ at } x = 0, f(x) = 3$$

$$f(-3) = 12, \quad f(5) = 28$$

So the image is $[3, 28]$

$$f^{-1}([12, 19])$$

$$12 \leq x^2 + 3 \leq 19 \text{ is true when } 3 \leq |x| \leq 4$$

$$\text{So, } f^{-1}([12, 19]) = [-4, -3] \cup [3, 4]$$

2

$$f = \{(1, 3), (2, 8), (3, 3), (4, 1), (5, 2), (6, 4), (7, 6)\}$$

$$f(\{1, 2, 3\}) = \{3, 8\}$$

$$f(\{4, 5, 6, 7\}) = \{1, 2, 4, 6\}$$

$$f(\emptyset) = \emptyset$$

No element maps to any of those outputs so $f^{-1}(\{0, 5, 9\}) = \emptyset$

$$f^{-1}(\{0, 3, 5, 9\}) = \{1, 3\}$$

10

First we prove $f^{-1}(Y \cap Z) \subseteq f^{-1}(Y) \cap f^{-1}(Z)$.

Let $a \in f^{-1}(Y \cap Z)$. By definition of preimage, this means $f(a) \in Y \cap Z$. Therefore $f(a) \in Y$ and $f(a) \in Z$.

Again using the definition of preimage, we get $a \in f^{-1}(Y)$ and $a \in f^{-1}(Z)$.

Hence $a \in f^{-1}(Y) \cap f^{-1}(Z)$, so $f^{-1}(Y \cap Z) \subseteq f^{-1}(Y) \cap f^{-1}(Z)$.

Next, the reverse inclusion $f^{-1}(Y) \cap f^{-1}(Z) \subseteq f^{-1}(Y \cap Z)$.

Let $a \in f^{-1}(Y) \cap f^{-1}(Z)$. Then $a \in f^{-1}(Y)$ and $a \in f^{-1}(Z)$, so $f(a) \in Y$ and $f(a) \in Z$.

Hence $f(a) \in Y \cap Z$, which means $a \in f^{-1}(Y \cap Z)$. Therefore $f^{-1}(Y) \cap f^{-1}(Z) \subseteq f^{-1}(Y \cap Z)$.

Since we have both inclusions, the two sets are equal: $f^{-1}(Y \cap Z) = f^{-1}(Y) \cap f^{-1}(Z)$.

1 Newtons Method

Derivative of $y = x^2 - x^3 + 2 \Rightarrow y' = 2x - 3x^2$

Start off with guess $n = 1.5$

$$1.5 - \frac{0.875}{-3.75} = 1.7\bar{3}$$

Now with $1.7\bar{3}$, rounded to 1.7333

$$1.7333 - \frac{-0.203074}{-5.54639} \approx 1.696686$$

With 1.696686

$$1.696686 - \frac{-0.00558021}{-5.24286} \approx 1.6956216$$

One more iteration for good measure, the intended number is $\equiv 1.69562076955986$

$$1.6956216 - \frac{-0.000004346649275}{-5.2341546312} \equiv 1.6956207695604 \text{ yeah thats close enough}$$